theories/iris/logrel/fundamental_kinding.v
@@ -1,0 +1,74 @@
+(* Fundamental theorem for the kind system:
+     well-kinded syntactic types are semantically well-kinded *)
+
+From iris.proofmode Require Import base tactics classes.
+From RichWasm Require Import layout syntax typing.
+From RichWasm.compiler Require Import codegen instrs modules util.
+From RichWasm.iris Require Import autowp gc.
+From RichWasm.iris.logrel Require Import relations.
+
+Set Bullet Behavior "Strict Subproofs".
+Set Default Goal Selector "!".
+
+Section FundamentalKinding.
+  Context `{Σ: gFunctors}.
+  Context `{!logrel_na_invs Σ}.
+  Context `{!wasmG Σ}.
+  Context `{!RichWasmGCG Σ}.
+
+  Variable sr : store_runtime.
+  Variable mr : module_runtime.
+  
+  Lemma sizity_sized_le_unsized σ :
+    sizity_interp (Σ:=Σ) (Sized σ) ⊑ sizity_interp Unsized.
+  Proof.
+    iIntros "%sv (%μ & %ws & %Hsv & %Hsz)".
+    iPureIntro.
+    do 2 eexists; split; eauto.
+    intros; congruence.
+  Qed.
+
+  Theorem kinding_sound F s__mem s__rep s__size se τ κ : 
+    has_kind F τ κ ->
+    subst_env_interp F s__mem s__rep s__size se
+    ⊢ kind_interp κ (value_interp sr se (subst_type s__mem s__rep s__size VarT τ)).
+  Proof.
+    intros Hkind. 
+    revert s__mem s__rep s__size se.
+    induction Hkind; intros; iIntros "Hsubst".
+    - admit.
+    - admit.
+    - admit.
+    - admit.
+    - admit.
+    - admit.
+    - admit.
+    - admit.
+      (* CHANGE to use true by construction refinement *)
+    - admit.
+    - admit.
+    - admit.
+    - admit.
+    - admit.
+    - admit.
+    - admit.
+    - admit.
+    - admit.
+    - admit.
+    - admit.
+    - admit.
+    - admit.
+    - admit.
+    - admit.
+    - admit.
+    - admit.
+    - admit.
+    - admit.
+    - admit.
+    - admit.
+    - admit.
+    - admit.
+  Admitted.
+
+End FundamentalKinding.
+
